meta/lakefile.lean
@@ -14,4 +14,5 @@ lean_lib «KanonMeta» where
 @[default_target]
 lean_lib «KanonMetaTests» where
   roots := #[`test.Regression, `test.Initiality, `test.InitialChain, `test.VectorConstruction,
-    `test.FinitaryConstruction, `test.FinitarySequence]
+    `test.FinitaryConstruction, `test.FinitarySequence,
+    `test.MuSyntax, `test.GeneratedMuNat, `test.MuNat]
